src/Iris/Algebra/GenMap.lean
@@ -1,0 +1,361 @@
+/-
+Copyright (c) 2025 Mario Carneiro. All rights reserved.
+Released under Apache 2.0 license as described in the file LICENSE.
+Authors: Markus de Medeiros
+-/
+import Iris.Algebra.OFE
+import Iris.Algebra.CMRA
+import Iris.Algebra.Updates
+
+namespace Iris
+open OFE
+
+section GenMap
+
+/- The OFE over gmaps is eqivalent to a non-depdenent discrete function to an `Option` type with a
+`Leibniz` OFE of keys, and an infinite number of unallocated elements.
+
+In this setting, the CMRA is always unital, and as a consquence the oFunctors do not require
+unitality in order to act as a `URFunctor(Contractive)`.
+
+GenMap is only intended to be used in the construction of the core IProp model. It is a stripped-down
+version of the generic heap constructions, which you should use instead. -/
+
+def alter [DecidableEq α] (f : α → β) (a : α) (b : β) : α → β :=
+  fun a' => if a = a' then b else f a'
+
+structure Enum (P : α → Prop) (enum : Nat → α) : Prop where
+  inc {n} : P (enum n)
+  inj {n m} : enum n = enum m → n = m
+
+def Poke [DecidableEq α] (enum : Nat → α) (n : Nat) : Nat → α :=
+  fun n' => if n' < n then enum n' else enum (n' + 1)
+
+def Infinite (P : α → Prop) : Prop := ∃ e, Enum P e
+
+def IsFree {β : α → Type _} (f : (a : α) → Option (β a)) : α → Prop := fun a => f a = none
+
+set_option grind.warning false
+theorem alter_isFree_infinite [DecidableEq α] {f : α → Option β} (H : Infinite (IsFree f)) :
+    Infinite (IsFree (alter f a b)) := by
+  rcases H with ⟨enum, Henum_inc, Henum_inj⟩
+  rcases Classical.em (∃ n₀, enum n₀ = a) with (⟨n₀, Hin⟩|Hout)
+  · refine ⟨Poke enum n₀, @fun n => ?_, @fun n m => ?_⟩
+    · simp [alter, IsFree]; split <;> rename_i h <;> revert h <;> simp [Poke]
+      · split <;> intro H <;> specialize Henum_inj (Hin ▸ H) <;> omega
+      · split <;> refine fun _ => Henum_inc
+    · simp [Poke]
+      split <;> split
+      all_goals intro H <;> specialize Henum_inj H <;> grind
+  · refine ⟨enum, @fun n => ?_, @fun n m Heq => ?_⟩
+    · simp only [not_exists] at Hout; specialize Hout n
+      simp only [IsFree, alter] at ⊢
+      split
+      · rename_i h; exact (Hout h.symm).elim
+      · exact Henum_inc
+    · exact Henum_inj Heq
+
+theorem Infinite.mono {P Q : α → Prop} (H : Infinite P) (Hmono : ∀ a, P a → Q a) : Infinite Q := by
+  rcases H with ⟨enum, Henum_inc, Henum_inj⟩
+  exact ⟨enum, Hmono (enum _) Henum_inc, Henum_inj⟩
+
+section GenMapImpl
+
+-- abbrev GenMap := { f : α → Option β // Infinite (IsFree f) }
+structure GenMap (α β : Type _) where
+  car : α → Option β
+
+nonrec def GenMap.alter [DecidableEq α] (g : GenMap α β) (a : α) (b : Option β) : GenMap α β where
+  car := alter g.car a b
+
+section OFE
+variable (α β : Type _) [OFE β]
+
+instance GenMap_instOFE : OFE (GenMap α β) where
+  Equiv := (·.car ≡ ·.car)
+  Dist n := (·.car ≡{n}≡ ·.car)
+  dist_eqv.refl _ := Dist.of_eq rfl
+  dist_eqv.symm := Dist.symm
+  dist_eqv.trans := Dist.trans
+  equiv_dist := equiv_dist
+  dist_lt := Dist.lt
+end OFE
+
+section CMRA
+
+variable (α β : Type _) [CMRA β]
+
+-- NB. Could use actual subtypes, but I will first attempt to do the subtyping on validity alone
+-- May make the OFunctors simpler because I just need to point them to GenMap instead
+-- of writing something new.
+-- Seems that the alter and alloc updates are still provable?
+instance instCMRA_GenMap : CMRA (GenMap α β) where
+  pcore x := Option.map GenMap.mk <| CMRA.pcore x.car
+  op x y := GenMap.mk (x.car • y.car)
+  ValidN n x := ✓{n} x.car ∧ (Infinite (IsFree x.car))
+  Valid x := ✓ x.car ∧ (Infinite (IsFree x.car))
+  op_ne.ne {_ _ _} H := CMRA.op_ne (α := α → Option β) |>.ne H
+  pcore_ne {n x y cx} H Hm := by
+    have Hm' : (CMRA.pcore x.car) = some cx.car := by
+      rcases h : (CMRA.pcore x.car)
+      · simp_all [h]
+      · simp_all [h]
+        rw [← Hm]
+    have H' : x.car ≡{n}≡ y.car := by exact H
+    rcases CMRA.pcore_ne H' Hm' with ⟨cy', Hcy'1, Hcy'2⟩
+    exact ⟨⟨cy'⟩, by simp [Hcy'1], Hcy'2⟩
+  validN_ne {n x y H} := by
+    refine fun ⟨Hv, ⟨e, Hf, Hi⟩⟩ => ⟨Dist.validN H |>.mp Hv, ?_⟩
+    refine ⟨e, @fun n => ?_, Hi⟩
+    specialize H (e n); specialize @Hf n; revert H Hf
+    cases _ : x.car (e n) <;> cases _ : y.car (e n) <;>
+    simp_all [IsFree, OFE.Dist, Option.Forall₂]
+  valid_iff_validN {x} := by
+    refine ⟨fun ⟨Hv, Hi⟩ n => ⟨Hv.validN, Hi⟩, fun H => ⟨?_, H 0 |>.2⟩⟩
+    exact CMRA.valid_iff_validN.mpr (H · |>.1)
+  validN_succ {x n} := fun ⟨Hv, Hi⟩ => ⟨CMRA.validN_succ Hv, Hi⟩
+  validN_op_left {n x y} := by
+    simp; rintro Hv Hf
+    refine ⟨CMRA.validN_op_left Hv, ?_⟩
+    refine Infinite.mono Hf (fun a => ?_)
+    simp [IsFree, CMRA.op, optionOp]
+    cases _ : x.car a <;> cases _ : y.car a  <;> simp
+  assoc {x y z} a := by
+    cases _ : x.car a <;> cases _ : y.car a <;> cases _ : z.car a <;>
+      simp_all [CMRA.op, OFE.Equiv, Option.Forall₂, optionOp]
+    exact CMRA.assoc
+  comm {x y} a := by
+    cases _ : x.car a <;> cases _ : y.car a <;>
+      simp_all [CMRA.op, OFE.Equiv, Option.Forall₂, optionOp]
+    exact CMRA.comm
+  pcore_op_left {x cx} H := by
+    rcases x with ⟨x⟩; rcases cx with ⟨cx⟩
+    have _ := CMRA.pcore_op_left (x := x) (cx := cx)
+    simp_all [OFE.Equiv]
+  pcore_idem {x cx} H := by
+    rcases x with ⟨x⟩; rcases cx with ⟨cx⟩
+    simp_all [OFE.Equiv, Option.Forall₂, Option.map]
+    apply CMRA.pcore_idem (x := x) (cx := cx)
+    simp [CMRA.pcore, H]
+  pcore_op_mono {x cx} := by
+    rcases x with ⟨x⟩; rcases cx with ⟨cx⟩; simp
+    refine fun H ⟨y⟩ => ?_
+    rcases CMRA.pcore_op_mono (x := x) (cx := cx) H y with ⟨cy, Hcy⟩
+    refine ⟨.mk cy, Hcy⟩
+  extend {n x y1 y2} := by
+    rintro ⟨Hv, _⟩ H
+    rcases CMRA.extend Hv H with ⟨z1, z2, _, _, _⟩
+    exists .mk z1
+    exists .mk z2
+
+instance instUCMRA_GenMap : UCMRA (GenMap Nat β) where
+  unit := GenMap.mk <| UCMRA.unit
+  unit_valid := ⟨fun _ => trivial, ⟨id, rfl, id⟩⟩
+  unit_left_id := by simp [CMRA.op, UCMRA.unit, optionOp]
+  pcore_unit := by simp [CMRA.pcore, UCMRA.unit, CMRA.core, optionCore]
+
+theorem GenMap.alter_valid [DecidableEq α] {g : GenMap α β} (Hb : ✓{n} b) (Hg : ✓{n} g) :
+    ✓{n} g.alter a b := by
+  rcases g with ⟨g⟩ <;> simp [GenMap.alter]
+  rcases Hg with ⟨Hv, Hi⟩
+  refine ⟨fun _ => ?_, alter_isFree_infinite Hi⟩
+  simp [Iris.alter] <;> split
+  · exact Hb
+  · exact Hv _
+
+theorem GenMap.valid_exists_fresh {g : GenMap α β} (Hv : ✓{n} g) : ∃ a : α, g.car a = none := by
+  rcases Hv with ⟨_, e, He_inc, _⟩
+  exact ⟨e 0, He_inc⟩
+
+end CMRA
+
+section OFunctors
+open COFE
+
+abbrev GenMapOF (C : Type _) (F : OFunctorPre) : OFunctorPre :=
+  fun A B _ _ => GenMap C (F A B)
+
+abbrev GenMap.lift [OFE α] [OFE β] (f : α -n> β) : GenMap T α -n> GenMap T β where
+  f g := .mk fun t => Option.map f (g.car t)
+  ne := sorry
+
+instance GenMapOF_instOFunctor (F : OFunctorPre) [OFunctor F] :
+    OFunctor (GenMapOF Nat F) where
+  cofe {A B _ _} := GenMap_instOFE Nat (F A B)
+  map f₁ f₂ := GenMap.lift <| OFunctor.map (F := F) f₁ f₂
+  map_ne.ne := sorry -- _ _ _ Hx _ _ Hy _ _  := by apply OFunctor.map_ne.ne Hx Hy
+  map_id := by sorry
+  map_comp := sorry -- by apply OFunctor.map_comp
+
+instance GenMapOF_instURFunctor (F : COFE.OFunctorPre) [RFunctor F] :
+    URFunctor (GenMapOF Nat F) where
+  map f g := {
+    toHom := GenMap.lift <| COFE.OFunctor.map f g
+    validN hv := by
+      let X := RFunctor.map (F := F) f g
+      dsimp [GenMap.lift]
+      sorry -- (URFunctor.map f g).validN (hv _)
+    pcore := sorry -- simpa [CMRA.pcore_eq_core] using (URFunctor.map f g).pcore _
+    op _ := sorry -- (URFunctor.map f g).op _ _
+  }
+  map_ne.ne := sorry -- COFE.OFunctor.map_ne.ne
+  map_id := sorry -- COFE.OFunctor.map_id
+  map_comp := sorry -- COFE.OFunctor.map_comp
+
+instance GenMapOF_instURFC {C} (F : COFE.OFunctorPre) [HURF : RFunctorContractive F] :
+    URFunctorContractive (GenMapOF C F) := sorry
+  -- map_contractive.1 h _ _ := URFunctorContractive.map_contractive.distLater_dist h _
+
+end OFunctors
+
+section updates
+
+-- Which gmap updates do we need?
+
+end updates
+
+
+/-
+Lemma insert_updateP (P : A → Prop) (Q : gmap K A → Prop) m i x :
+  x ~~>: P →
+  (∀ y, P y → Q (<[i:=y]>m)) →
+  <[i:=x]>m ~~>: Q.
+Proof.
+  intros Hx%option_updateP' HP; apply cmra_total_updateP=> n mf Hm.
+  destruct (Hx n (Some (mf !! i))) as ([y|]&?&?); try done.
+  { by generalize (Hm i); rewrite lookup_op; simplify_map_eq. }
+  exists (<[i:=y]> m); split; first by auto.
+  intros j; move: (Hm j)=>{Hm}; rewrite !lookup_op=>Hm.
+  destruct (decide (i = j)); simplify_map_eq/=; auto.
+Qed.
+Lemma insert_updateP' (P : A → Prop) m i x :
+  x ~~>: P → <[i:=x]>m ~~>: λ m', ∃ y, m' = <[i:=y]>m ∧ P y.
+Proof. eauto using insert_updateP. Qed.
+Lemma insert_update m i x y : x ~~> y → <[i:=x]>m ~~> <[i:=y]>m.
+Proof. rewrite !cmra_update_updateP; eauto using insert_updateP with subst. Qed.
+
+Lemma singleton_updateP (P : A → Prop) (Q : gmap K A → Prop) i x :
+  x ~~>: P → (∀ y, P y → Q {[ i := y ]}) → {[ i := x ]} ~~>: Q.
+Proof. apply insert_updateP. Qed.
+Lemma singleton_updateP' (P : A → Prop) i x :
+  x ~~>: P → {[ i := x ]} ~~>: λ m, ∃ y, m = {[ i := y ]} ∧ P y.
+Proof. apply insert_updateP'. Qed.
+Lemma singleton_update i (x y : A) : x ~~> y → {[ i := x ]} ~~> {[ i := y ]}.
+Proof. apply insert_update. Qed.
+
+Lemma delete_update m i : m ~~> delete i m.
+Proof.
+  apply cmra_total_update=> n mf Hm j; destruct (decide (i = j)); subst.
+  - move: (Hm j). rewrite !lookup_op lookup_delete_eq left_id.
+    apply cmra_validN_op_r.
+  - move: (Hm j). by rewrite !lookup_op lookup_delete_ne.
+Qed.
+
+
+
+
+
+Section freshness.
+  Local Set Default Proof Using "Type*".
+  Context `{!Infinite K}.
+  Lemma alloc_updateP_strong_dep (Q : gmap K A → Prop) (I : K → Prop) m (f : K → A) :
+    pred_infinite I →
+    (∀ i, m !! i = None → I i → ✓ (f i)) →
+    (∀ i, m !! i = None → I i → Q (<[i:=f i]>m)) → m ~~>: Q.
+  Proof.
+    move=> /(pred_infinite_set I (C:=gset K)) HP ? HQ.
+    apply cmra_total_updateP. intros n mf Hm.
+    destruct (HP (dom (m ⋅ mf))) as [i [Hi1 Hi2]].
+    assert (m !! i = None).
+    { eapply not_elem_of_dom. revert Hi2.
+      rewrite dom_op not_elem_of_union. naive_solver. }
+    exists (<[i:=f i]>m); split.
+    - by apply HQ.
+    - rewrite insert_singleton_op //.
+      rewrite -assoc -insert_singleton_op; last by eapply not_elem_of_dom.
+    apply insert_validN; [apply cmra_valid_validN|]; auto.
+  Qed.
+  Lemma alloc_updateP_strong (Q : gmap K A → Prop) (I : K → Prop) m x :
+    pred_infinite I →
+    ✓ x → (∀ i, m !! i = None → I i → Q (<[i:=x]>m)) → m ~~>: Q.
+  Proof.
+    move=> HP ? HQ. eapply (alloc_updateP_strong_dep _ _ _ (λ _, x)); eauto.
+  Qed.
+  Lemma alloc_updateP (Q : gmap K A → Prop) m x :
+    ✓ x → (∀ i, m !! i = None → Q (<[i:=x]>m)) → m ~~>: Q.
+  Proof.
+    move=>??.
+    eapply (alloc_updateP_strong _ (λ _, True));
+    eauto using pred_infinite_True.
+  Qed.
+  Lemma alloc_updateP_cofinite (Q : gmap K A → Prop) (J : gset K) m x :
+    ✓ x → (∀ i, m !! i = None → i ∉ J → Q (<[i:=x]>m)) → m ~~>: Q.
+  Proof.
+    eapply alloc_updateP_strong.
+    apply (pred_infinite_set (C:=gset K)).
+    intros E. exists (fresh (J ∪ E)).
+    apply not_elem_of_union, is_fresh.
+  Qed.
+
+  (* Variants without the universally quantified Q, for use in case that is an evar. *)
+  Lemma alloc_updateP_strong_dep' m (f : K → A) (I : K → Prop) :
+    pred_infinite I →
+    (∀ i, m !! i = None → I i → ✓ (f i)) →
+    m ~~>: λ m', ∃ i, I i ∧ m' = <[i:=f i]>m ∧ m !! i = None.
+  Proof. eauto using alloc_updateP_strong_dep. Qed.
+  Lemma alloc_updateP_strong' m x (I : K → Prop) :
+    pred_infinite I →
+    ✓ x → m ~~>: λ m', ∃ i, I i ∧ m' = <[i:=x]>m ∧ m !! i = None.
+  Proof. eauto using alloc_updateP_strong. Qed.
+  Lemma alloc_updateP' m x :
+    ✓ x → m ~~>: λ m', ∃ i, m' = <[i:=x]>m ∧ m !! i = None.
+  Proof. eauto using alloc_updateP. Qed.
+  Lemma alloc_updateP_cofinite' m x (J : gset K) :
+    ✓ x → m ~~>: λ m', ∃ i, i ∉ J ∧ m' = <[i:=x]>m ∧ m !! i = None.
+  Proof. eauto using alloc_updateP_cofinite. Qed.
+End freshness.
+
+Lemma alloc_unit_singleton_updateP (P : A → Prop) (Q : gmap K A → Prop) u i :
+  ✓ u → LeftId (≡) u (⋅) →
+  u ~~>: P → (∀ y, P y → Q {[ i := y ]}) → ∅ ~~>: Q.
+Proof.
+  intros ?? Hx HQ. apply cmra_total_updateP=> n gf Hg.
+  destruct (Hx n (gf !! i)) as (y&?&Hy).
+  { move:(Hg i). rewrite !left_id.
+    case: (gf !! i)=>[x|]; rewrite /= ?left_id //.
+    intros; by apply cmra_valid_validN. }
+  exists {[ i := y ]}; split; first by auto.
+  intros i'; destruct (decide (i' = i)) as [->|].
+  - rewrite lookup_op lookup_singleton_eq.
+    move:Hy; case: (gf !! i)=>[x|]; rewrite /= ?right_id //.
+  - move:(Hg i'). by rewrite !lookup_op lookup_singleton_ne // !left_id.
+Qed.
+Lemma alloc_unit_singleton_updateP' (P: A → Prop) u i :
+  ✓ u → LeftId (≡) u (⋅) →
+  u ~~>: P → ∅ ~~>: λ m, ∃ y, m = {[ i := y ]} ∧ P y.
+Proof. eauto using alloc_unit_singleton_updateP. Qed.
+Lemma alloc_unit_singleton_update (u : A) i (y : A) :
+  ✓ u → LeftId (≡) u (⋅) → u ~~> y → (∅:gmap K A) ~~> {[ i := y ]}.
+Proof.
+  rewrite !cmra_update_updateP;
+    eauto using alloc_unit_singleton_updateP with subst.
+Qed.
+-/
+
+-- def GenMapOF (C : Type _) (F : C → COFE.OFunctorPre) : COFE.OFunctorPre :=
+--   fun A B => { f : (c : C) → OptionOF (F c) A B // Infinite (IsFree f) }
+
+-- TODO: CMRA instances, updates for alloc + modify, urFunctor instance for when F is always an rFunctor
+-- Functor merges
+--    urFunctorOptionOF [RFunctor F] : URFunctor (OptionOF F) where
+-- instance urFunctorContractiveOptionOF [RFunctorContractive F] : URFunctorContractive (OptionOF F) where
+--    DiscreteFunOF_URFC {C} (F : C → COFE.OFunctorPre) [HURF : ∀ c, URFunctorContractive (F c)] :
+-- So it should expect ∀ c, (RFunctorContractive c)
+
+-- instance instURFunctor_GenMapOF {F : C → COFE.OFunctorPre} [∀ c, RFunctorContractive (F c)] :
+--     URFunctor (GenMapOF C F) :=
+--   sorry
+
+end GenMapImpl
+
+end GenMap
